Calculus/MultiStaged/Monad/Identity.v
@@ -14,7 +14,7 @@ Require Import "Calculus/MultiStaged/Monad".
   Monadic translation with identity monad sends a calculus to itself.
   It is the simplest possible monad. We prove that identity monad
   verifies required algebraic properties.
-**)
+*)
 
 Module IdentityMonad (R:Replacement) (T:ReplacementCalculus R) <: (Monad R T).
 
@@ -44,36 +44,33 @@ Module IdentityMonad (R:Replacement) (T:ReplacementCalculus R) <: (Monad R T).
 
   (** Var Translation *)
   Definition cast_var (v:var) : var := v.
-  Definition is_cast_var (x:var) : Prop := exists y, cast_var y = x.
 
   (** Abstract Reduction step *)
   Definition astep : relation state := sstep 0.
 
   (** Substitution Properties *)
   Lemma ssubst_ret :
-    forall (n:nat) (ss:StageSet.t) (x:var) (e v:expr),
-     is_cast_var x ->
-     ssubst n ss x (ret e) v = ret (ssubst n ss x e v).
+    forall (n:nat) (ss:StageSet.t) (x:S.var) (e v:expr),
+     ssubst n ss (cast_var x) (ret e) v = ret (ssubst n ss (cast_var x) e v).
   Proof.
     reflexivity.
   Qed.
 
   Lemma ssubst_bind :
-    forall (n:nat) (ss:StageSet.t) (x:var) (e1 v:expr) (f: expr -> expr),
-     is_cast_var x ->
-     ((fun v2 => ssubst n ss x (f v2) v) = 
-       fun v2 => f (ssubst n ss x v2 v)) ->
-     ssubst n ss x (bind e1 f) v = 
-       bind (ssubst n ss x e1 v) f.
+    forall (n:nat) (ss:StageSet.t) (x:S.var) (e1 v:expr) (e2: expr -> expr),
+     ((fun v2 => ssubst n ss (cast_var x) (e2 v2) v) = 
+       fun v2 => e2 (ssubst n ss (cast_var x) v2 v)) ->
+     ssubst n ss (cast_var x) (bind e1 e2) v = 
+       bind (ssubst n ss (cast_var x) e1 v) e2.
   Proof.
     intros.
     unfold bind.
-    assert(forall v2, ((fun v2 : expr => ssubst n ss x (f v2) v) v2 =
-     (fun v2 : expr => f (ssubst n ss x v2 v)) v2)).
+    assert(forall v2, ((fun v2 : expr => ssubst n ss (cast_var x) (e2 v2) v) v2 =
+     (fun v2 : expr => e2 (ssubst n ss (cast_var x) v2 v)) v2)).
       apply equal_f.
       assumption.
-    specialize (H1 e1).
-    simpl in H1.
+    specialize (H0 e1).
+    simpl in H0.
     assumption.
   Qed.
 
@@ -83,29 +80,27 @@ Module IdentityMonad (R:Replacement) (T:ReplacementCalculus R) <: (Monad R T).
        bind e1 (fun v2 => e2 (ssubst n ss x v2 v)).*)
 
   Lemma ssubst_eabs :
-    forall (n:nat) (ss:StageSet.t) (x y:var) (e v:expr),
-     is_cast_var x ->
-     ssubst n ss x (cast_eabs y e) v = 
-     cast_eabs y (ssubst n (if beq_var x y 
-        then (StageSet.add n ss) else ss) x e v).
+    forall (n:nat) (ss:StageSet.t) (x y:S.var) (e v:expr),
+     ssubst n ss (cast_var x) (cast_eabs (cast_var y) e) v = 
+     cast_eabs (cast_var y) (ssubst n (if S.beq_var x y 
+        then (StageSet.add n ss) else ss) (cast_var x) e v).
   Proof.
     reflexivity.
   Qed.
 
   Lemma ssubst_efix :
-    forall (n:nat) (ss:StageSet.t) (x f y:var) (e v:expr),
-     is_cast_var x ->
-     ssubst n ss x (cast_efix f y e) v = 
-     cast_efix f y (ssubst n (if orb (beq_var x f) (beq_var x y) 
-        then (StageSet.add n ss) else ss) x e v).
+    forall (n:nat) (ss:StageSet.t) (x f y:S.var) (e v:expr),
+     ssubst n ss (cast_var x) (cast_efix (cast_var f) (cast_var y) e) v = 
+     cast_efix (cast_var f) (cast_var y) (ssubst n (if orb (S.beq_var x f) (S.beq_var x y) 
+        then (StageSet.add n ss) else ss) (cast_var x) e v).
   Proof.
     reflexivity.
   Qed.
 
   Lemma ssubst_eref :
-    forall (n:nat) (ss:StageSet.t) (x:var) (e v:expr),
-     is_cast_var x ->
-     ssubst n ss x (cast_eref e) v = cast_eref (ssubst n ss x e v).
+    forall (n:nat) (ss:StageSet.t) (x:S.var) (e v:expr),
+     ssubst n ss (cast_var x) (cast_eref e) v
+       = cast_eref (ssubst n ss (cast_var x) e v).
   Proof.
     reflexivity.
   Qed.
